Reorganize code

theories/seqcalc.v
@@ -1,89 +1,9 @@
 From Coq Require Import ssreflect.
 From stdpp Require Import prelude.
 From iris_mod.bi Require Import bi.
+From bunched Require Export syntax interp.
 
-Declare Scope bunch_scope.
-Delimit Scope bunch_scope with B.
-
-(** * Syntax and sequence calculus for BI *)
-
-Definition atom := nat.
-
-(** ** Formulas and bunches *)
-Inductive formula : Type :=
-| TOP
-| EMP
-| BOT
-| ATOM (A : atom)
-| CONJ (ϕ ψ : formula)
-| SEP (ϕ ψ : formula)
-| IMPL (ϕ ψ : formula)
-| WAND (ϕ ψ : formula)
-.
-
-Inductive bunch : Type :=
-| frml (ϕ : formula)
-| top : bunch
-| empty : bunch
-| comma (Δ1 Δ2 : bunch)
-| semic (Δ1 Δ2 : bunch)
-.
-
-Local Infix ";," := semic (at level 80, right associativity) : bunch_scope.
-Local Infix ",," := comma (at level 80, right associativity) : bunch_scope.
-
-(** "Collapse" internalizes the bunch as a formula. *)
-Fixpoint collapse (Δ : bunch) : formula :=
-  match Δ with
-  | top => TOP
-  | empty => EMP
-  | frml ϕ => ϕ
-  | (Δ ,, Δ')%B => SEP (collapse Δ) (collapse Δ')
-  | (Δ ;, Δ')%B => CONJ (collapse Δ) (collapse Δ')
-  end.
-
-(** Bunched contexts with a hole *)
-Inductive bunch_ctx_item : Type :=
-| CtxCommaL (Δ2 : bunch)    (* Δ ↦ Δ , Δ2 *)
-| CtxCommaR (Δ1 : bunch)    (* Δ ↦ Δ1, Δ *)
-| CtxSemicL (Δ2 : bunch)    (* Δ ↦ Δ; Δ2 *)
-| CtxSemicR (Δ1 : bunch)    (* Δ ↦ Δ1; Δ *)
-.
-
-Definition bunch_ctx := list bunch_ctx_item.
-
-Definition fill_item (C : bunch_ctx_item) (Δ : bunch) : bunch :=
-  match C with
-  | CtxCommaL Δ2 => Δ ,, Δ2
-  | CtxCommaR Δ1 => Δ1 ,, Δ
-  | CtxSemicL Δ2 => Δ ;, Δ2
-  | CtxSemicR Δ1 => Δ1 ;, Δ
-  end%B.
-
-Definition fill (Π : bunch_ctx) (Δ : bunch) : bunch :=
-  foldl (flip fill_item) Δ Π.
-
-(** ** Bunch equivalence *)
-(** Equivalence on bunches is defined to be the least congruence
-      that satisfies the monoidal laws for (empty and comma) and (top
-      and semicolon). *)
-Inductive bunch_equiv : bunch → bunch → Prop :=
-| BE_refl Δ : Δ =? Δ
-| BE_sym Δ1 Δ2 : Δ1 =? Δ2 → Δ2 =? Δ1
-| BE_trans Δ1 Δ2 Δ3 : Δ1 =? Δ2 → Δ2 =? Δ3 → Δ1 =? Δ3
-| BE_cong C Δ1 Δ2 : Δ1 =? Δ2 → fill C Δ1 =? fill C Δ2
-| BE_comma_unit_l Δ : (empty ,, Δ)%B =? Δ
-| BE_comma_comm Δ1 Δ2  : (Δ1 ,, Δ2)%B =? (Δ2 ,, Δ1)%B
-| BE_comma_assoc Δ1 Δ2 Δ3  : (Δ1 ,, (Δ2 ,, Δ3))%B =? ((Δ1 ,, Δ2) ,, Δ3)%B
-| BE_semic_unit_l Δ : (top ;, Δ)%B =? Δ
-| BE_semic_comm Δ1 Δ2  : (Δ1 ;, Δ2)%B =? (Δ2 ;, Δ1)%B
-| BE_semic_assoc Δ1 Δ2 Δ3  : (Δ1 ;, (Δ2 ;, Δ3))%B =? ((Δ1 ;, Δ2) ;, Δ3)%B
-where "Δ =? Γ" := (bunch_equiv Δ%B Γ%B).
-
-(** Register [bunch_equiv] as [(≡)] *)
-Global Instance equiv_bunch_equiv : Equiv bunch := bunch_equiv.
-
-(** ** Sequent calculus itself *)
+(** * Sequent calculus  *)
 Reserved Notation "P ⊢ᴮ Q" (at level 99, Q at level 200, right associativity).
 Inductive proves : bunch → formula → Prop :=
 (* structural *)
@@ -139,83 +59,10 @@ Inductive proves : bunch → formula → Prop :=
     fill C (Δ ;, frml (IMPL ϕ ψ)) ⊢ᴮ χ
 where "Δ ⊢ᴮ ϕ" := (proves Δ%B ϕ%B).
 
-(** ** Alternative representation of decomposition of bunches *)
-(** We have an inductive type that characterizes when a bunch can be
-  decomposed into a context and a sub-bunch. This essentially gives an
-  us an inductive reasoning principle for equations [fill Π Δ = Δ']. *)
-Inductive bunch_decomp :
-  bunch → bunch_ctx → bunch → Prop :=
-| decomp_id Δ : bunch_decomp Δ [] Δ
-| decomp_comma_1 Δ1 Δ2 Π Δ :
-    bunch_decomp Δ1 Π Δ →
-    bunch_decomp (Δ1,,Δ2)%B (Π ++ [CtxCommaL Δ2]) Δ
-| decomp_comma_2 Δ1 Δ2 Π Δ :
-    bunch_decomp Δ2 Π Δ →
-    bunch_decomp (Δ1,,Δ2)%B (Π ++ [CtxCommaR Δ1]) Δ
-| decomp_semic_1 Δ1 Δ2 Π Δ :
-    bunch_decomp Δ1 Π Δ →
-    bunch_decomp (Δ1;,Δ2)%B (Π ++ [CtxSemicL Δ2]) Δ
-| decomp_semic_2 Δ1 Δ2 Π Δ :
-    bunch_decomp Δ2 Π Δ →
-    bunch_decomp (Δ1;,Δ2)%B (Π ++ [CtxSemicR Δ1]) Δ.
-
 (** * Properties *)
-
-Lemma fill_app (Π Π' : bunch_ctx) (Δ : bunch) :
-  fill (Π ++ Π') Δ = fill Π' (fill Π Δ).
-Proof. by rewrite /fill foldl_app. Qed.
 
 (** Registering the right typeclasses for rewriting purposes. *)
 
-Global Instance equivalence_bunch_equiv : Equivalence ((≡@{bunch})).
-Proof.
-  repeat split.
-  - intro x. econstructor.
-  - intros x y Hxy. by econstructor.
-  - intros x y z Hxy Hyz. by econstructor.
-Qed.
-
-Global Instance comma_comm : Comm (≡) comma.
-Proof. intros X Y. apply BE_comma_comm. Qed.
-Global Instance semic_comm : Comm (≡) semic.
-Proof. intros X Y. apply BE_semic_comm. Qed.
-Global Instance comma_assoc : Assoc (≡) comma.
-Proof. intros X Y Z. apply BE_comma_assoc. Qed.
-Global Instance semic_assoc : Assoc (≡) semic.
-Proof. intros X Y Z. apply BE_semic_assoc. Qed.
-Global Instance comma_left_id : LeftId (≡) empty comma.
-Proof. intros X. by econstructor. Qed.
-Global Instance comma_right_id : RightId (≡) empty comma.
-Proof. intros X. rewrite comm. by econstructor. Qed.
-Global Instance semic_left_id : LeftId (≡) top semic.
-Proof. intros X. by econstructor. Qed.
-Global Instance semic_right_id : RightId (≡) top semic.
-Proof. intros X. rewrite comm. by econstructor. Qed.
-
-Global Instance fill_proper C : Proper ((≡) ==> (≡)) (fill C).
-Proof. intros X Y. apply BE_cong. Qed.
-
-Global Instance comma_proper : Proper ((≡) ==> (≡) ==> (≡)) comma.
-Proof.
-  intros Δ1 Δ2 H Δ1' Δ2' H'.
-  change ((fill [CtxCommaL Δ1'] Δ1) ≡ (fill [CtxCommaL Δ2'] Δ2)).
-  etrans.
-  { eapply BE_cong; eauto. }
-  simpl.
-  change ((fill [CtxCommaR Δ2] Δ1') ≡ (fill [CtxCommaR Δ2] Δ2')).
-  eapply BE_cong; eauto.
-Qed.
-
-Global Instance semic_proper : Proper ((≡) ==> (≡) ==> (≡)) semic.
-Proof.
-  intros Δ1 Δ2 H Δ1' Δ2' H'.
-  change ((fill [CtxSemicL Δ1'] Δ1) ≡ (fill [CtxSemicL Δ2'] Δ2)).
-  etrans.
-  { eapply BE_cong; eauto. }
-  simpl.
-  change ((fill [CtxSemicR Δ2] Δ1') ≡ (fill [CtxSemicR Δ2] Δ2')).
-  eapply BE_cong; eauto.
-Qed.
 Global Instance proves_proper : Proper ((≡) ==> (=) ==> (≡)) proves.
 Proof.
   intros D1 D2 HD ϕ ? <-.
@@ -224,118 +71,30 @@ Proof.
   - eapply BI_Equiv; [ symmetry | ]; eauto.
 Qed.
 
-(** [bunch_decomp Δ' Π Δ] completely characterizes [fill Π Δ = Δ'] *)
-Lemma bunch_decomp_correct Δ Π Δ' :
-  bunch_decomp Δ Π Δ' → Δ = fill Π Δ'.
-Proof. induction 1; rewrite ?fill_app /= //; try by f_equiv. Qed.
-
-Lemma bunch_decomp_complete' Π Δ' :
-  bunch_decomp (fill Π Δ') Π Δ'.
+Theorem seq_interp_sound {PROP : bi} (s : atom → PROP)
+        Δ ϕ : (Δ ⊢ᴮ ϕ) → seq_interp PROP s Δ ϕ.
 Proof.
-  revert Δ'. remember (reverse Π) as Πr.
-  revert Π HeqΠr.
-  induction Πr as [|HΠ Πr]=>Π HeqΠr.
-  { assert (Π = []) as ->.
-    {  by eapply (inj reverse). }
-    simpl. intros. econstructor. }
-  intros Δ'.
-  assert (Π = reverse Πr ++ [HΠ]) as ->.
-  { by rewrite -reverse_cons HeqΠr reverse_involutive. }
-  rewrite fill_app /=.
-  revert Δ'.
-  induction HΠ=>Δ' /=; econstructor; eapply IHΠr; by rewrite reverse_involutive.
+  induction 1; unfold seq_interp; simpl; eauto; try rewrite -IHproves.
+  all: try by apply bunch_interp_fill_mono.
+  - by rewrite -H.
+  - apply bunch_interp_fill_mono; simpl.
+      by rewrite bi.and_elim_l.
+  - apply bunch_interp_fill_mono; simpl.
+    apply bi.and_intro; eauto.
+  - by rewrite IHproves1 IHproves2.
+  - by apply bi.wand_intro_r.
+  - rewrite -IHproves2.
+    apply bunch_interp_fill_mono; simpl.
+    rewrite IHproves1. apply bi.wand_elim_r.
+  - induction C as [|C Π IH]; simpl.
+    { apply bi.False_elim. }
+    rewrite -IH.
+    destruct C; simpl; apply bunch_interp_fill_mono; simpl.
+    all: by rewrite ?left_absorb ?right_absorb.
+  - apply bi.True_intro.
+  - by rewrite IHproves1 IHproves2.
+  - by apply bi.impl_intro_r.
+  - rewrite -IHproves2.
+    apply bunch_interp_fill_mono; simpl.
+    rewrite IHproves1. apply bi.impl_elim_r.
 Qed.
-
-Lemma bunch_decomp_complete Δ Π Δ' :
-  (fill Π Δ' = Δ) →
-  bunch_decomp Δ Π Δ'.
-Proof. intros <-. apply bunch_decomp_complete'. Qed.
-
-Lemma fill_is_frml Π Δ ϕ :
-  fill Π Δ = frml ϕ →
-  Π = [] ∧ Δ = frml ϕ.
-Proof.
-  revert Δ. induction Π as [| F C IH]=>Δ; first by eauto.
-  destruct F ; simpl ; intros H1 ;
-    destruct (IH _ H1) as [HC HΔ] ; by simplify_eq/=.
-Qed.
-
-Lemma bunch_decomp_app C C0 Δ Δ0 :
-  bunch_decomp Δ C0 Δ0 →
-  bunch_decomp (fill C Δ) (C0 ++ C) Δ0.
-Proof.
-  revert Δ Δ0 C0.
-  induction C as [|F C]=>Δ Δ0 C0.
-  { simpl. by rewrite app_nil_r. }
-  intros HD.
-  replace (C0 ++ F :: C) with ((C0 ++ [F]) ++ C); last first.
-  { by rewrite -assoc. }
-  apply IHC. destruct F; simpl; by econstructor.
-Qed.
-
-Lemma bunch_decomp_ctx C C' Δ ϕ :
-  bunch_decomp (fill C Δ) C' (frml ϕ) →
-  ((∃ C0, bunch_decomp Δ C0 (frml ϕ) ∧ C' = C0 ++ C) ∨
-   (∃ (C0 C1 : bunch → bunch_ctx),
-       (∀ Δ Δ', fill (C0 Δ) Δ' = fill (C1 Δ') Δ) ∧
-       (∀ Δ', fill (C1 Δ') Δ = fill C' Δ') ∧
-       (∀ A, bunch_decomp (fill C A) (C0 A) (frml ϕ)))).
-Proof.
-  revert Δ C'.
-  induction C as [|F C]=>Δ C'; simpl.
-  { remember (frml ϕ) as Γ1. intros Hdec.
-    left. eexists. rewrite right_id. split; done. }
-  simpl. intros Hdec.
-  destruct (IHC _ _ Hdec) as [IH|IH].
-  - destruct IH as [C0 [HC0 HC]].
-    destruct F; simpl in *.
-    + inversion HC0; simplify_eq/=.
-      * left. eexists; split; eauto.
-        rewrite -assoc //.
-      * right.
-        exists (λ A, (Π ++ [CtxCommaR A]) ++ C).
-        exists (λ A, ([CtxCommaL (fill Π A)] ++ C)).
-        repeat split.
-        { intros A B. by rewrite /= -!assoc /= !fill_app. }
-        { intros A. by rewrite /= -!assoc /= !fill_app. }
-        { intros A. apply bunch_decomp_app. by econstructor. }
-    + inversion HC0; simplify_eq/=.
-      * right.
-        exists (λ A, (Π ++ [CtxCommaL A]) ++ C).
-        exists (λ A, ([CtxCommaR (fill Π A)] ++ C)).
-        repeat split.
-        { intros A B. by rewrite /= -!assoc /= !fill_app. }
-        { intros A. by rewrite /= -!assoc /= !fill_app. }
-        { intros A. apply bunch_decomp_app. by econstructor. }
-      * left. eexists; split; eauto.
-        rewrite -assoc //.
-    + inversion HC0; simplify_eq/=.
-      * left. eexists; split; eauto.
-        rewrite -assoc //.
-      * right.
-        exists (λ A, (Π ++ [CtxSemicR A]) ++ C).
-        exists (λ A, ([CtxSemicL (fill Π A)] ++ C)).
-        repeat split.
-        { intros A B. by rewrite /= -!assoc /= !fill_app. }
-        { intros A. by rewrite /= -!assoc /= !fill_app. }
-        { intros A. apply bunch_decomp_app. by econstructor. }
-    + inversion HC0; simplify_eq/=.
-      * right.
-        exists (λ A, (Π ++ [CtxSemicL A]) ++ C).
-        exists (λ A, ([CtxSemicR (fill Π A)] ++ C)).
-        repeat split.
-        { intros A B. by rewrite /= -!assoc /= !fill_app. }
-        { intros A. by rewrite /= -!assoc /= !fill_app. }
-        { intros A. apply bunch_decomp_app. by econstructor. }
-      * left. eexists; split; eauto.
-        rewrite -assoc //.
-  - right.
-    destruct IH as (C0 & C1 & HC0 & HC1 & HC).
-    exists (λ A, C0 (fill_item F A)), (λ A, F::C1 A). repeat split.
-    { intros A B. simpl. rewrite -HC0 //. }
-    { intros B. rewrite -HC1 //. }
-    intros A. apply HC.
-Qed.
-
-Notation "Δ ';,' Γ" := (semic Δ%B Γ%B) (at level 80, right associativity) : bunch_scope.
-Notation "Δ ',,' Γ" := (comma Δ%B Γ%B) (at level 80, right associativity) : bunch_scope.
