theories/syntax.v
@@ -1,0 +1,140 @@
+(* Formulas, bunches *)
+From Coq Require Import ssreflect.
+From stdpp Require Import prelude gmap fin_sets.
+From iris_mod.bi Require Import bi.
+
+Declare Scope bunch_scope.
+Delimit Scope bunch_scope with B.
+
+(** * Formulas and bunches *)
+Definition atom := nat.
+
+Inductive formula : Type :=
+| TOP
+| EMP
+| BOT
+| ATOM (A : atom)
+| CONJ (ϕ ψ : formula)
+| SEP (ϕ ψ : formula)
+| IMPL (ϕ ψ : formula)
+| WAND (ϕ ψ : formula)
+.
+
+Inductive bunch : Type :=
+| frml (ϕ : formula)
+| top : bunch
+| empty : bunch
+| comma (Δ1 Δ2 : bunch)
+| semic (Δ1 Δ2 : bunch)
+.
+
+Notation "Δ ';,' Γ" := (semic Δ%B Γ%B) (at level 80, right associativity) : bunch_scope.
+Notation "Δ ',,' Γ" := (comma Δ%B Γ%B) (at level 80, right associativity) : bunch_scope.
+
+(** ** Bunched contexts with a hole *)
+Inductive bunch_ctx_item : Type :=
+| CtxCommaL (Δ2 : bunch)    (* Δ ↦ Δ , Δ2 *)
+| CtxCommaR (Δ1 : bunch)    (* Δ ↦ Δ1, Δ *)
+| CtxSemicL (Δ2 : bunch)    (* Δ ↦ Δ; Δ2 *)
+| CtxSemicR (Δ1 : bunch)    (* Δ ↦ Δ1; Δ *)
+.
+
+Definition bunch_ctx := list bunch_ctx_item.
+
+Definition fill_item (F : bunch_ctx_item) (Δ : bunch) : bunch :=
+  match F with
+  | CtxCommaL Δ2 => Δ ,, Δ2
+  | CtxCommaR Δ1 => Δ1 ,, Δ
+  | CtxSemicL Δ2 => Δ ;, Δ2
+  | CtxSemicR Δ1 => Δ1 ;, Δ
+  end%B.
+
+Definition fill (Π : bunch_ctx) (Δ : bunch) : bunch :=
+  foldl (flip fill_item) Δ Π.
+
+(** "Collapse" internalizes the bunch as a formula. *)
+Fixpoint collapse (Δ : bunch) : formula :=
+  match Δ with
+  | top => TOP
+  | empty => EMP
+  | frml ϕ => ϕ
+  | (Δ ,, Δ')%B => SEP (collapse Δ) (collapse Δ')
+  | (Δ ;, Δ')%B => CONJ (collapse Δ) (collapse Δ')
+  end.
+
+(** ** Bunch equivalence *)
+(** Equivalence on bunches is defined to be the least congruence
+      that satisfies the monoidal laws for (empty and comma) and (top
+      and semicolon). *)
+Inductive bunch_equiv : bunch → bunch → Prop :=
+| BE_refl Δ : Δ =? Δ
+| BE_sym Δ1 Δ2 : Δ1 =? Δ2 → Δ2 =? Δ1
+| BE_trans Δ1 Δ2 Δ3 : Δ1 =? Δ2 → Δ2 =? Δ3 → Δ1 =? Δ3
+| BE_cong C Δ1 Δ2 : Δ1 =? Δ2 → fill C Δ1 =? fill C Δ2
+| BE_comma_unit_l Δ : (empty ,, Δ)%B =? Δ
+| BE_comma_comm Δ1 Δ2  : (Δ1 ,, Δ2)%B =? (Δ2 ,, Δ1)%B
+| BE_comma_assoc Δ1 Δ2 Δ3  : (Δ1 ,, (Δ2 ,, Δ3))%B =? ((Δ1 ,, Δ2) ,, Δ3)%B
+| BE_semic_unit_l Δ : (top ;, Δ)%B =? Δ
+| BE_semic_comm Δ1 Δ2  : (Δ1 ;, Δ2)%B =? (Δ2 ;, Δ1)%B
+| BE_semic_assoc Δ1 Δ2 Δ3  : (Δ1 ;, (Δ2 ;, Δ3))%B =? ((Δ1 ;, Δ2) ;, Δ3)%B
+where "Δ =? Γ" := (bunch_equiv Δ%B Γ%B).
+
+(** Register [bunch_equiv] as [(≡)] *)
+Global Instance equiv_bunch_equiv : Equiv bunch := bunch_equiv.
+
+(** * Properties *)
+
+Global Instance equivalence_bunch_equiv : Equivalence ((≡@{bunch})).
+Proof.
+  repeat split.
+  - intro x. econstructor.
+  - intros x y Hxy. by econstructor.
+  - intros x y z Hxy Hyz. by econstructor.
+Qed.
+
+Global Instance comma_comm : Comm (≡) comma.
+Proof. intros X Y. apply BE_comma_comm. Qed.
+Global Instance semic_comm : Comm (≡) semic.
+Proof. intros X Y. apply BE_semic_comm. Qed.
+Global Instance comma_assoc : Assoc (≡) comma.
+Proof. intros X Y Z. apply BE_comma_assoc. Qed.
+Global Instance semic_assoc : Assoc (≡) semic.
+Proof. intros X Y Z. apply BE_semic_assoc. Qed.
+Global Instance comma_left_id : LeftId (≡) empty comma.
+Proof. intros X. by econstructor. Qed.
+Global Instance comma_right_id : RightId (≡) empty comma.
+Proof. intros X. rewrite comm. by econstructor. Qed.
+Global Instance semic_left_id : LeftId (≡) top semic.
+Proof. intros X. by econstructor. Qed.
+Global Instance semic_right_id : RightId (≡) top semic.
+Proof. intros X. rewrite comm. by econstructor. Qed.
+
+Global Instance fill_proper Π : Proper ((≡) ==> (≡)) (fill Π).
+Proof. intros X Y. apply BE_cong. Qed.
+
+Global Instance comma_proper : Proper ((≡) ==> (≡) ==> (≡)) comma.
+Proof.
+  intros Δ1 Δ2 H Δ1' Δ2' H'.
+  change ((fill [CtxCommaL Δ1'] Δ1) ≡ (fill [CtxCommaL Δ2'] Δ2)).
+  etrans.
+  { eapply BE_cong; eauto. }
+  simpl.
+  change ((fill [CtxCommaR Δ2] Δ1') ≡ (fill [CtxCommaR Δ2] Δ2')).
+  eapply BE_cong; eauto.
+Qed.
+
+Global Instance semic_proper : Proper ((≡) ==> (≡) ==> (≡)) semic.
+Proof.
+  intros Δ1 Δ2 H Δ1' Δ2' H'.
+  change ((fill [CtxSemicL Δ1'] Δ1) ≡ (fill [CtxSemicL Δ2'] Δ2)).
+  etrans.
+  { eapply BE_cong; eauto. }
+  simpl.
+  change ((fill [CtxSemicR Δ2] Δ1') ≡ (fill [CtxSemicR Δ2] Δ2')).
+  eapply BE_cong; eauto.
+Qed.
+
+Lemma fill_app (Π Π' : bunch_ctx) (Δ : bunch) :
+  fill (Π ++ Π') Δ = fill Π' (fill Π Δ).
+Proof. by rewrite /fill foldl_app. Qed.
+
