theories/terms.v
@@ -1,0 +1,77 @@
+(* Bunched terms *)
+From Equations Require Import Equations.
+From Coq Require Import ssreflect.
+From stdpp Require Import prelude gmap fin_sets.
+From iris_mod.bi Require Import bi.
+From bunched Require Import syntax.
+
+(** * Bunched terms *)
+Inductive bterm (var : Type) : Type :=
+| Var (x : var)
+| TComma (T1 T2 : bterm var)
+.
+Arguments Var {_} x.
+Arguments TComma {_} T1 T2.
+
+Global Instance bterm_fmap : FMap bterm :=
+  fix go _ _ f T { struct T } := let _ : FMap _ := go in
+  match T with
+  | Var x => Var (f x)
+  | TComma T1 T2 => TComma (f <$> T1) (f <$> T2)
+  end.
+
+Equations term_fv `{!EqDecision V,!Countable V} (T : bterm V) : gset V :=
+  term_fv (Var x) := {[ x ]};
+  term_fv (TComma T1 T2) := term_fv T1 ∪ term_fv T2;
+.
+
+Equations linear_bterm `{!EqDecision V,!Countable V}
+  (T : bterm V) : Prop :=
+  linear_bterm (Var x) := True;
+  linear_bterm (TComma T1 T2) :=
+    term_fv T1 ## term_fv T2 ∧
+    linear_bterm T1 ∧ linear_bterm T2.
+
+Fixpoint bterm_ctx_act `{!EqDecision V,!Countable V}
+         (T : bterm V) (Δs : V → bunch) : bunch :=
+  match T with
+  | Var v => Δs v
+  | TComma T1 T2 => bterm_ctx_act T1 Δs,, bterm_ctx_act T2 Δs
+  end%B.
+
+Fixpoint bterm_alg_act {PROP : bi} `{!EqDecision V,!Countable V}
+         (T : bterm V) (Xs : V → PROP) : PROP :=
+  match T with
+  | Var v => Xs v
+  | TComma T1 T2 => bterm_alg_act T1 Xs ∗ bterm_alg_act T2 Xs
+  end%I.
+
+(** A semimorphism between BI algebras is a function that preserves ∗ and ∧ *)
+Class SemiMorph {A B : bi} (f : A → B) :=
+  { smor_sep (X Y : A) : (f X ∗ f Y)%I ≡ (f (X ∗ Y))%I; }.
+
+Lemma bterm_fmap_compose {A B C} (f : A → B) (g : B → C) (T : bterm A) :
+  (g ∘ f) <$> T = g <$> (f <$> T).
+Proof.
+  induction T; simpl; auto.
+  rewrite IHT1 IHT2 //.
+Qed.
+
+Lemma bterm_ctx_act_fv `{!EqDecision V,!Countable V} (T : bterm V) Δs Γs :
+  (∀ i : V, i ∈ term_fv T → Δs i = Γs i) →
+  bterm_ctx_act T Δs = bterm_ctx_act T Γs.
+Proof.
+  induction T; simp term_fv ; simpl.
+  - set_solver.
+  - set_unfold. intros H.
+    rewrite IHT1; eauto. rewrite IHT2; eauto.
+Qed.
+
+Lemma bterm_morph_commute {A B : bi} `{!EqDecision V, !Countable V}
+      (T : bterm V) (Xs : V → A) (f : A → B) `{!SemiMorph f}:
+  f (bterm_alg_act (PROP:=A) T Xs) ≡ bterm_alg_act (PROP:=B) T (f ∘ Xs).
+Proof.
+  induction T; simpl; first reflexivity.
+  rewrite -IHT1 -IHT2. by rewrite smor_sep.
+Qed.
+
